LeanBF/Core/Instruction.lean
@@ -1,0 +1,32 @@
+/-
+Copyright (c) 2026 Bangyen Pham. All rights reserved.
+Released under Apache 2.0 license as described in the file LICENSE.
+Authors: Bangyen Pham
+-/
+
+/-!
+# Brainfuck Instructions
+
+## Main definitions
+
+* `Instruction`: The eight Brainfuck commands plus the bracketed loop.
+* `Program`: A Brainfuck program (a list of instructions).
+-/
+
+namespace LeanBF
+
+/-- Brainfuck instructions -/
+inductive Instruction where
+  | inc_ptr : Instruction  -- `>`
+  | dec_ptr : Instruction  -- `<`
+  | inc_val : Instruction  -- `+`
+  | dec_val : Instruction  -- `-`
+  | loop    : List Instruction → Instruction -- `[` and `]`
+  | read    : Instruction  -- `,`
+  | write   : Instruction  -- `.`
+  deriving Repr, BEq
+
+/-- A Brainfuck program is a list of instructions -/
+abbrev Program := List Instruction
+
+end LeanBF
