Tests/Compiler.lean
@@ -1,0 +1,30 @@
+/-
+Copyright (c) 2026 Bangyen Pham. All rights reserved.
+Released under Apache 2.0 license as described in the file LICENSE.
+Authors: Bangyen Pham
+-/
+import LeanBF.Core.Compiler
+
+/-!
+# Compiler Tests
+-/
+
+namespace LeanBF.Tests
+
+open LeanBF
+
+example : Compiler.movePtr 1 1 = [] :=
+  rfl
+
+example : Compiler.movePtr 0 1 = [.inc_ptr] :=
+  rfl
+
+example : Compiler.movePtr 2 0 = [.dec_ptr, .dec_ptr] :=
+  rfl
+
+example : Compiler.compileInstr (.inc1 1) =
+    List.replicate 2 .inc_ptr ++ [.inc_val, .dec_ptr] ++
+    List.replicate 256 .dec_val ++ [.inc_val, .dec_ptr] :=
+  rfl
+
+end LeanBF.Tests
