Tests/Minsky.lean
@@ -1,0 +1,34 @@
+/-
+Copyright (c) 2026 Bangyen Pham. All rights reserved.
+Released under Apache 2.0 license as described in the file LICENSE.
+Authors: Bangyen Pham
+-/
+import LeanBF.Core.Minsky
+
+/-!
+# Minsky Tests
+-/
+
+namespace LeanBF.Tests
+
+open LeanBF
+
+example : Minsky.step [] { pc := 0, c1 := 0, c2 := 0 } = none :=
+  rfl
+
+example : Minsky.step [.halt] { pc := 0, c1 := 0, c2 := 0 } = none :=
+  rfl
+
+example : Minsky.step [.inc1 1] { pc := 0, c1 := 0, c2 := 0 } =
+    some { pc := 1, c1 := 1, c2 := 0 } :=
+  rfl
+
+example : Minsky.step [.jzdec1 0 1] { pc := 0, c1 := 2, c2 := 0 } =
+    some { pc := 1, c1 := 1, c2 := 0 } :=
+  rfl
+
+example : Minsky.step [.jzdec2 0 1] { pc := 0, c1 := 0, c2 := 2 } =
+    some { pc := 1, c1 := 0, c2 := 1 } :=
+  rfl
+
+end LeanBF.Tests
