Tests/Semantics.lean
@@ -1,0 +1,28 @@
+/-
+Copyright (c) 2026 Bangyen Pham. All rights reserved.
+Released under Apache 2.0 license as described in the file LICENSE.
+Authors: Bangyen Pham
+-/
+import LeanBF.Core.Semantics
+
+/-!
+# Semantics Tests
+-/
+
+namespace LeanBF.Tests
+
+open LeanBF
+
+example : step [] State.mkEmpty = none :=
+  rfl
+
+example : step [.inc_val] State.mkEmpty = some ([], State.incVal State.mkEmpty) :=
+  rfl
+
+example : step [.write] State.mkEmpty = some ([], { State.mkEmpty with output := [0] }) :=
+  rfl
+
+example : RunsTo ([], State.mkEmpty) State.mkEmpty :=
+  RunsTo.halt State.mkEmpty
+
+end LeanBF.Tests
