Tests/State.lean
@@ -1,0 +1,34 @@
+/-
+Copyright (c) 2026 Bangyen Pham. All rights reserved.
+Released under Apache 2.0 license as described in the file LICENSE.
+Authors: Bangyen Pham
+-/
+import LeanBF.Core.State
+
+/-!
+# State Tests
+-/
+
+namespace LeanBF.Tests
+
+open LeanBF
+
+example : State.ptr State.mkEmpty = 0 :=
+  rfl
+
+example : State.input State.mkEmpty = [] :=
+  rfl
+
+example : State.output State.mkEmpty = [] :=
+  rfl
+
+example : State.currentVal State.mkEmpty = 0 :=
+  rfl
+
+example : State.incPtr State.mkEmpty = { State.mkEmpty with ptr := 1 } :=
+  rfl
+
+example : State.currentVal (State.incVal State.mkEmpty) = 1 :=
+  rfl
+
+end LeanBF.Tests
